\documentclass[11pt,a4paper]{article}
\usepackage[utf8x]{inputenc}
\usepackage[T1]{fontenc}
\usepackage{mathptmx}
\usepackage{graphicx}
\usepackage[pdftex,linkcolor=black,pdfborder={0 0 0}]{hyperref} % Format links for pdf
\usepackage{calc} % To reset the counter in the document after title page
\usepackage{enumitem} % Includes lists
\usepackage{caption}
\captionsetup[figure]{font=small,labelfont=small,labelfont=bf}
\usepackage{subcaption}
\usepackage{amsmath}
\usepackage{amssymb}
\usepackage{amsfonts}
\usepackage{fancyvrb,newverbs,xcolor}
\usepackage{verbatim}
\definecolor{cverbbg}{gray}{0.93}

\newenvironment{lcverbatim}
 {\SaveVerbatim{cverb}}
 {\endSaveVerbatim
  \flushleft\fboxrule=0pt\fboxsep=.5em
  \colorbox{cverbbg}{%
    \makebox[\dimexpr\linewidth-2\fboxsep][l]{\BUseVerbatim{cverb}}%
  }
  \endflushleft
}

\renewcommand\thesection{Task \arabic{section}}
\renewcommand\thesubsection{\alph{subsection}.)}
\renewcommand\thesubsubsection{\Roman{subsubsection}:}

\frenchspacing
\linespread{1.2}
\usepackage[a4paper, lmargin=0.12\paperwidth, rmargin=0.12\paperwidth, tmargin=0.05\paperheight, bmargin=0.1\paperheight]{geometry}

\usepackage[all]{nowidow} % Tries to remove widows
\usepackage[protrusion=true,expansion=true]{microtype}

\title{Exercise 9}
\author{Kai Schneider}
\date{\today}

\begin{document} 

\maketitle

\section{Reinforce on the Cart-Pole}

\subsection{}

softmax: $\;\; \pi(a|s,\theta) = \frac{e^{h(s,a,\theta)}}{\sum_{b}e^{h(s,a,\theta)}}$ \\

\flushleft
linear features: $\;\; h(s,a,\theta) = \theta_{a}^{T}s$ \\

\vspace{10pt}

for the 2 actions space $a\in\{0, 1\}$ of the cart pole this results in  
$\;\; \pi(a|s,\theta) = \frac{e^{\theta_{a}^{T}s}}{e^{\theta_{0}^{T}s} + e^{\theta_{1}^{T}s}} \;\;$ for the softmax function.
With state $s=(p, \dot{p}, \alpha, \dot{\alpha})^{T}\in\mathbb{R}^4$ follows $\theta\in\mathbb{R}^4$ \\

This results for the given actions in: 

\vspace{5pt}

\begin{center}
$\pi(a=0|s,\theta) = \frac{e^{\theta_{0}^{T}s}}{e^{\theta_{0}^{T}s} + e^{\theta_{1}^{T}s}} \;\;$ and 
$\;\; \pi(a=1|s,\theta) = \frac{e^{\theta_{1}^{T}s}}{e^{\theta_{0}^{T}s} + e^{\theta_{1}^{T}s}}$
\end{center}

\vspace{5pt}

These can be rewritten as a sigmoid function:

\begin{align*}
\pi(a=0|s,\theta) &= \frac{e^{\theta_{0}^{T}s}} {e^{\theta_{0}^{T}s} + e^{\theta_{1}^{T}s}} \\
                  &= \frac{e^{\theta_{0}^{T}s}} {e^{\theta_{0}^{T}s} \bigl( e^{\theta_{1}^{T}s - \theta_{0}^{T}s} + 1 \bigr)} \\
                  &=  \frac{1} {e^{\theta_{1}^{T}s - \theta_{0}^{T}s} + 1} \\
                  &=  \sigma(\theta_{0}^{T}s - \theta_{1}^{T}s) \\
                  &=  \sigma(s^{T}(\theta_{0} - \theta_{1}))
\end{align*}

similar for $\;\; \pi(a=1|s,\theta) =  \sigma(s^{T}(\theta_{1} - \theta_{0}))$

\vspace{5pt}

Also due to $\sigma(z) = \frac{1}{1+e^{-z}} = \frac{e^{z}}{1+e^{z}}$ we have

\begin{align*}
  \pi(a=0|s,\theta) &= 1 - \pi(a=1|s,\theta) \\
                    &= 1 - \sigma(s^{T}(\theta_{1} - \theta_{0}))
\end{align*}
  
and vice versa

\begin{center}
  $\pi(a=1|s,\theta) = 1 - \sigma(s^{T}(\theta_{0} - \theta_{1}))$
\end{center}

\vspace{5pt}

With $\sigma'(z) = \sigma(z) \bigl( 1 - \sigma(z) \bigr)$ being the derivative of the sigma function we get: \\

\begin{align*}
  \nabla_{\theta_{0}} \pi(a=0|s,\theta) &= \sigma(s^{T}(\theta_{0} - \theta_{1})) \bigl( 1 -  \sigma(s^{T}(\theta_{0} - \theta_{1})) \bigr)s \\
  \nabla_{\theta_{1}} \pi(a=0|s,\theta) &= -\sigma(s^{T}(\theta_{0} - \theta_{1})) \bigl( 1 -  \sigma(s^{T}(\theta_{0} - \theta_{1})) \bigr)s \\
  \nabla_{\theta_{1}} \pi(a=1|s,\theta) &= \sigma(s^{T}(\theta_{1} - \theta_{0})) \bigl( 1 -  \sigma(s^{T}(\theta_{1} - \theta_{0})) \bigr)s \\
  \nabla_{\theta_{0}} \pi(a=1|s,\theta) &= -\sigma(s^{T}(\theta_{1} - \theta_{0})) \bigl( 1 -  \sigma(s^{T}(\theta_{1} - \theta_{0})) \bigr)s
\end{align*}


\subsection{}

The derivate $\nabla_{\theta} \log \pi(a=0|s,\theta)$ can be calculated in a similar fashion:


\begin{align*}
  \nabla_{\theta_{0}} \log \pi(a=0|s,\theta) &= \frac{1}{\pi(a=0|s,\theta)} 
                  \sigma(s^{T}(\theta_{0} - \theta_{1})) \bigl( 1 -  \sigma(s^{T}(\theta_{0} - \theta_{1})) \bigr)s \\
  &= \frac{1}{\sigma(s^{T}(\theta_{0} - \theta_{1}))} 
  \sigma(s^{T}(\theta_{0} - \theta_{1})) \bigl( 1 -  \sigma(s^{T}(\theta_{0} - \theta_{1})) \bigr)s \\
  &= \bigl( 1 -  \sigma(s^{T}(\theta_{0} - \theta_{1})) \bigr)s \\
  \nabla_{\theta_{1}} \log \pi(a=0|s,\theta) &= \bigl( 1 -  \sigma(s^{T}(\theta_{0} - \theta_{1})) \bigr)(-s)
\end{align*}

and 

\begin{align*}
  \nabla_{\theta_{1}} \log \pi(a=1|s,\theta) &=  \bigl( 1 -  \sigma(s^{T}(\theta_{1} - \theta_{0})) \bigr)s \\
  \nabla_{\theta_{0}} \log \pi(a=1|s,\theta) &=  \bigl( 1 -  \sigma(s^{T}(\theta_{1} - \theta_{0})) \bigr)(-s) \\
\end{align*}

This can again be rewritten with the results from \textbf{a.)}:


\begin{align*}
  \nabla_{\theta} \log \pi(a=0|s,\theta) &=  \bigl( 1 -  \sigma(s^{T}(\theta_{0} - \theta_{1})) \bigr)s \\
                                         &= \sigma(s^{T}(\theta_{1} - \theta_{0}))s \\
\end{align*}

and

\begin{align*}
  \nabla_{\theta} \log \pi(a=1|s,\theta) &=  \bigl( 1 -  \sigma(s^{T}(\theta_{1} - \theta_{0})) \bigr)s \\
                                         &= \sigma(s^{T}(\theta_{0} - \theta_{1}))s \\
\end{align*}


















\end{document}

